lib/Lib.Rational.fsti
@@ -4,6 +4,8 @@ module Math = FStar.Math.Lemmas
 
 open FStar.Calc
 open FStar.Mul
+open FStar.Seq
+open Lib.Seq
 
 type rat = (int & pos)
 
@@ -18,7 +20,7 @@ let eq_refl (a: rat) : Lemma (ensures a =$ a) = ()
 let eq_sym (a b: rat): Lemma
   (requires a =$ b)
   (ensures b =$ a)
-  [SMTPat (a =$ b)] = ()
+  (* [SMTPat (a =$ b)] *) = ()
 
 let eq_trans (a b c: rat): Lemma
   (requires a =$ b /\ b =$ c)
@@ -28,7 +30,7 @@ let eq_trans (a b c: rat): Lemma
 let eq_req (a b: rat): Lemma
   (requires a == b)
   (ensures a =$ b)
-  [SMTPat (a == b)] = ()
+  (* [SMTPat (a == b)] *) = ()
 
 let (<=$) (a b: rat): bool = num a * den b <= num b * den a
 unfold let (>=$) (a b: rat): bool = b <=$ a
@@ -36,19 +38,19 @@ unfold let (>=$) (a b: rat): bool = b <=$ a
 let le_eq (a b a' b': rat): Lemma
   (requires a =$ a' /\ b =$ b' /\ a <=$ b)
   (ensures a' <=$ b')
-  [SMTPat (a =$ a'); SMTPat (b =$ b'); SMTPat (a <=$ b)] = ()
+  (* [SMTPat (a =$ a'); SMTPat (b =$ b'); SMTPat (a <=$ b)] *) = ()
 
 let le_refl (a: rat) : Lemma (ensures a <=$ a) = ()
 
 let le_antisym (a b: rat): Lemma
   (requires a <=$ b /\ b <=$ a)
   (ensures a =$ b)
-  [SMTPat (a <=$ b); SMTPat (b <=$ a)] = ()
+  (* [SMTPat (a <=$ b); SMTPat (b <=$ a)] *) = ()
 
 let le_trans (a b c: rat): Lemma
   (requires a <=$ b /\ b <=$ c)
   (ensures a <=$ c)
-  [SMTPat (a <=$ b); SMTPat (b <=$ c)] = ()
+  (* [SMTPat (a <=$ b); SMTPat (b <=$ c)] *) = ()
 
 let (<$) (a b: rat) = num a * den b < num b * den a
 unfold let (>$) (a b: rat) = b <$ a
@@ -56,27 +58,27 @@ unfold let (>$) (a b: rat) = b <$ a
 let lt_eq_l (a b a': rat): Lemma
   (requires a =$ a' /\ a <$ b)
   (ensures a' <$ b)
-  [SMTPat (a =$ a'); SMTPat (a <$ b)] = ()
+  (* [SMTPat (a =$ a'); SMTPat (a <$ b)] *) = ()
 
 let lt_eq_r (a b b': rat): Lemma
   (requires b =$ b' /\ a <$ b)
   (ensures a <$ b')
-  [SMTPat (b =$ b'); SMTPat (a <$ b)] = ()
+  (* [SMTPat (b =$ b'); SMTPat (a <$ b)] *) = ()
 
 let lt_not_eq (a b: rat) : Lemma
   (requires a <$ b)
   (ensures a <> b)
-  [SMTPat (a <$ b)] = ()
+  (* [SMTPat (a <$ b)] *) = ()
 
 let lt_trans (a b c: rat): Lemma
   (requires a <$ b /\ b <$ c)
   (ensures a <$ c)
-  [SMTPat (a <$ b); SMTPat (b <$ c)] = ()
+  (* [SMTPat (a <$ b); SMTPat (b <$ c)] *) = ()
 
 let lt_le_trans (a b c: rat): Lemma
   (requires a <$ b /\ b <=$ c)
   (ensures a <$ c)
-  [SMTPat (a <$ b); SMTPat (b <=$ c)] = ()
+  (* [SMTPat (a <$ b); SMTPat (b <=$ c)] *) = ()
 
 let (+$) (a b: rat): Tot rat =
   (num a * den b + num b * den a, den a * den b)
@@ -96,15 +98,15 @@ let plus_eq_r (a b b': rat): Lemma
 
 let plus_comm (a b: rat): Lemma
   (ensures a +$ b =$ b +$ a)
-  [SMTPat (a +$ b)] = ()
+  (* [SMTPat (a +$ b)] *) = ()
 
 let plus_zero_l (a: rat): Lemma
   (ensures zero +$ a =$ a)
-  [SMTPat (zero +$ a)] = ()
+  (* [SMTPat (zero +$ a)] *) = ()
 
 let plus_zero_r (a: rat): Lemma
   (ensures a +$ zero =$ a)
-  [SMTPat (a +$ zero)] = ()
+  (* [SMTPat (a +$ zero)] *) = ()
 
 let plus_non_zero_l (a b: rat): Lemma
   (requires zero <$ a)
@@ -113,7 +115,14 @@ let plus_non_zero_l (a b: rat): Lemma
 #set-options "--z3refresh --z3rlimit 1024 --fuel 0 --ifuel 0 --z3seed 12"
 val plus_assoc: a: rat -> b: rat -> c: rat -> Lemma
   (ensures (a +$ b) +$ c =$ a +$ (b +$ c))
-  [SMTPatOr [[SMTPat ((a +$ b) +$ c)]; [SMTPat (a +$ (b +$ c))]]]
+  (* [SMTPatOr [[SMTPat ((a +$ b) +$ c)]; [SMTPat (a +$ (b +$ c))]]] *)
+
+let (-$) (a b: rat): Tot rat = (num a * den b - num b * den a, den a * den b)
+
+let sub_eq (a b: rat): Lemma
+  (requires a =$ b)
+  (ensures a -$ b =$ zero)
+  (* [SMTPat (a -$ b =$ zero)] *) = ()
 
 let op_Star_Dollar (a b: rat): Tot rat = (num a * num b, den a * den b)
 
@@ -122,35 +131,33 @@ let common_factor_cancel (a: pos) (r: rat): Lemma
 
 let mul_zero_l (a: rat): Lemma
   (ensures a *$ zero =$ zero)
-  [SMTPat (a *$ zero)] = ()
+  (* [SMTPat (a *$ zero)] *) = ()
 
 let mul_zero_r (a: rat): Lemma
   (ensures zero *$ a =$ zero)
-  [SMTPat (zero *$ a)] = ()
+  (* [SMTPat (zero *$ a)] *) = ()
 
 let mul_comm (a b: rat): Lemma
   (ensures a *$ b =$ b *$ a)
-  [SMTPat (a *$ b)] = ()
+  (* [SMTPat (a *$ b)] *) = ()
 
 let mul_assoc (a b c: rat): Lemma
   (ensures (a *$ b) *$ c =$ a *$ (b *$ c))
-  [SMTPatOr [[SMTPat ((a *$ b) *$ c)]; [SMTPat (a *$ (b *$ c))]]] =
+  (* [SMTPatOr [[SMTPat ((a *$ b) *$ c)]; [SMTPat (a *$ (b *$ c))]]] *) =
   assert((a *$ b) *$ c =$ a *$ (b *$ c))
 
 val distributivity_add_left: a: rat -> b: rat -> c: rat -> Lemma
   (ensures (a *$ b) +$ (a *$ c) =$ a *$ (b +$ c))
 
-let mul_eq_l (a b a': rat): Lemma
+val mul_eq_l: a: rat -> b: rat -> a': rat -> Lemma
   (requires a =$ a')
   (ensures a *$ b =$ a' *$ b)
-  [SMTPat (a =$ a'); SMTPat (a' *$ b)] =
-  assert_norm(a *$ b =$ a' *$ b)
+  (* [SMTPat (a =$ a'); SMTPat (a' *$ b)] *)
 
-let mul_eq_r (a b b': rat): Lemma
+val mul_eq_r: a: rat -> b: rat -> b': rat -> Lemma
   (requires b =$ b')
   (ensures a *$ b =$ a *$ b')
-  [SMTPat (b =$ b'); SMTPat (a *$ b')] =
-  assert_norm(a *$ b =$ a *$ b')
+  (* [SMTPat (b =$ b'); SMTPat (a *$ b')] *)
 
 let of_int (a: int): rat = (a, 1)
 
@@ -158,54 +165,117 @@ let rec sigma (i: nat) (j: nat{i <= j}) (f: (k: nat{i <= k /\ k <= j}) -> rat):
   Tot rat (decreases j - i) =
   if i = j then f i else f i +$ sigma (i + 1) j f
 
-#push-options "--fuel 1"
-let rec sigma_mul_distributivity (i j: nat) (c: rat) (f g: (k: nat{i <= k /\ k <= j}) -> rat): Lemma
-  (requires i <= j /\ (forall k. f k = c *$ g k))
-  (ensures sigma i j f =$ c *$ sigma i j g)
-  (decreases j - i) =
-  if i < j then begin
-    sigma_mul_distributivity (i + 1) j c f g;
-    distributivity_add_left c (g i) (sigma (i + 1) j g)
-  end
+// #push-options "--fuel 1"
+// let rec sigma_mul_distributivity (i j: nat) (c: rat) (f g: (k: nat{i <= k /\ k <= j}) -> rat): Lemma
+//   (requires i <= j /\ (forall k. f k = c *$ g k))
+//   (ensures sigma i j f =$ c *$ sigma i j g)
+//   (decreases j - i) =
+//   if i < j then begin
+//     sigma_mul_distributivity (i + 1) j c f g;
+//     distributivity_add_left c (g i) (sigma (i + 1) j g)
+//   end
 
-let rec sigma_split (i j k: nat) (f: (l: nat{i <= l /\ l <= k}) -> rat): Lemma
-  (requires i <= j /\ j + 1 <= k)
-  (ensures sigma i k f =$ sigma i j f +$ sigma (j + 1) k f)
-  (decreases k - i) =
-  match k - i with
-  | 1 -> ()
-  | _ -> if i < j then sigma_split (i + 1) j k f
+// let rec sigma_split (i j k: nat) (f: (l: nat{i <= l /\ l <= k}) -> rat): Lemma
+//   (requires i <= j /\ j + 1 <= k)
+//   (ensures sigma i k f =$ sigma i j f +$ sigma (j + 1) k f)
+//   (decreases k - i) =
+//   match k - i with
+//   | 1 -> ()
+//   | _ -> if i < j then sigma_split (i + 1) j k f
 
-let rec sigma_gt_zero (i j: nat) (f: (k: nat{i <= k /\ k <= j}) -> rat): Lemma
-  (requires i <= j /\ (forall k. f k >$ zero))
-  (ensures sigma i j f >$ zero)
-  (decreases j - i) =
-  match j - i with
-  | 0 -> ()
-  | _ -> sigma_gt_zero (i + 1) j f
+// let rec sigma_gt_zero (i j: nat) (f: (k: nat{i <= k /\ k <= j}) -> rat): Lemma
+//   (requires i <= j /\ (forall k. f k >$ zero))
+//   (ensures sigma i j f >$ zero)
+//   (decreases j - i) =
+//   match j - i with
+//   | 0 -> ()
+//   | _ -> sigma_gt_zero (i + 1) j f
 
-let plus_non_zero_r (a b: rat): Lemma
-  (requires zero <$ a)
-  (ensures b <$ b +$ a) = ()
+// let plus_non_zero_r (a b: rat): Lemma
+//   (requires zero <$ a)
+//   (ensures b <$ b +$ a) = ()
   
-let sigma_pos_lt (i j k: nat) (f: (l: nat{i <= l /\ l <= k}) -> rat): Lemma
-  (requires i <= j /\ j < k /\ (forall l. f l >$ zero))
-  (ensures sigma i j f <$ sigma i k f) =
-  sigma_split i j k f;
-  sigma_gt_zero i j f;
-  sigma_gt_zero (j + 1) k f;
-  plus_non_zero_r (sigma (j + 1) k f) (sigma i j f)
+// let sigma_pos_lt (i j k: nat) (f: (l: nat{i <= l /\ l <= k}) -> rat): Lemma
+//   (requires i <= j /\ j < k /\ (forall l. f l >$ zero))
+//   (ensures sigma i j f <$ sigma i k f) =
+//   sigma_split i j k f;
+//   sigma_gt_zero i j f;
+//   sigma_gt_zero (j + 1) k f;
+//   plus_non_zero_r (sigma (j + 1) k f) (sigma i j f)
 
-let rec sigma_extensionality (i j: nat) (f g: (l: nat{i <= l /\ l <= j}) -> rat): Lemma
-  (requires i <= j /\ (forall k. i <= k /\ k <= j ==> f k =$ g k))
-  (ensures sigma i j f =$ sigma i j g)
-  (decreases j - i)
-  [SMTPat (sigma i j f =$ sigma i j g)] =
-  match j - i with
-  | 0 -> ()
-  | _ -> sigma_extensionality (i + 1) j f g
-#pop-options
+// let rec sigma_extensionality (i j: nat) (f g: (l: nat{i <= l /\ l <= j}) -> rat): Lemma
+//   (requires i <= j /\ (forall k. i <= k /\ k <= j ==> f k =$ g k))
+//   (ensures sigma i j f =$ sigma i j g)
+//   (decreases j - i)
+//   [SMTPat (sigma i j f =$ sigma i j g)] =
+//   match j - i with
+//   | 0 -> ()
+//   | _ -> sigma_extensionality (i + 1) j f g
+
+// #push-options "--ifuel 1"
+// let rec sigma_snoc (#t: eqtype) (s: seq t) (i: nat) (a: t) (f: t -> rat): Lemma
+//   (requires length s > 0 /\ i <= length s - 1)
+//   (ensures
+//     sigma i (length (snoc s a) - 2) (fun k -> f (snoc s a).[k]) =$
+//     sigma i (length s - 1) (fun k -> f s.[k]))
+//   (decreases length s - i) =
+//   let f' = fun k -> f (snoc s a).[k] in
+//   if i = length s - 1 then
+//     ()
+//   else
+//     calc (=$) {
+//       sigma i (length (snoc s a) - 2) f';
+//       =${}
+//       f s.[i] +$ sigma (i + 1) (length (snoc s a) - 2) f';
+//       =${
+//         calc (=$) {
+//           sigma (i + 1) (length (snoc s a) - 2) f';
+//           =${sigma_snoc s (i + 1) a f}
+//           sigma (i + 1) (length s - 1) (fun k -> f s.[k]);
+//         }
+//       }
+//       f s.[i] +$ sigma (i + 1) (length s - 1) (fun k -> f s.[k]);
+//     }
+// #pop-options
+// #pop-options
 
 let pow2_subtraction (a b: nat): Lemma
   (requires a >= b)
   (ensures (pow2 (a - b), 1) =$ (pow2 a, pow2 b)) = Math.pow2_plus (a - b) b
+
+let qpow2 (n: int): Tot rat =
+  match n >= 0 with
+  | true -> (pow2 n, 1)
+  | false -> (1, pow2 (-n <: nat))
+
+val qpow2_double_sum: n: int -> Lemma
+  (ensures qpow2 n +$ qpow2 n =$ qpow2 (n + 1))
+  [SMTPat (qpow2 n +$ qpow2 n)]
+
+let qpow2_mult_even (n: int) (m: nat): Lemma
+  (requires m % 2 == 0)
+  (ensures qpow2 n *$ (of_int m) =$ qpow2 (n + 1) *$ (of_int (m / 2))) =
+  if n < 0 then
+    calc (=$) {
+      qpow2 n *$ (of_int m);
+      =={}
+      (m, pow2 (-n));
+      =${Math.Lemmas.pow2_double_mult (-n - 1)}
+      (m / 2, (pow2 (-(n + 1))));
+      =${}
+      (1, (pow2 (-(n + 1)))) *$ (m / 2, 1);
+      =={assert_norm(pow2 0 == 1)}
+      qpow2 (n + 1) *$ of_int (m / 2);
+    }
+  else
+    calc (=$) {
+      qpow2 n *$ (of_int m);
+      =={}
+      (pow2 n * m, 1);
+      =={}
+      (pow2 n * 2 * (m / 2), 1);
+      =={Math.Lemmas.pow2_double_mult n}
+      (pow2 (n + 1) * (m / 2), 1);
+      =={}
+      qpow2 (n + 1) *$ of_int (m / 2);
+    }
